examples/mw/MWHeader.v
@@ -93,7 +93,7 @@ Section PROOF.
   (******************************* MW ****************************)
   Definition main_spec: fspec :=
     mk_simple (fun (_: unit) =>
-                 ((fun varg o => ⌜varg = ([]: list val)↑ ∧ o = ord_top⌝ ** OwnM Init),
+                 ((fun varg o => ⌜varg = ([]: list val)↑ ∧ o = ord_top⌝ ** OwnM Init ** OwnM (mw_state Maps.empty)),
                   (fun vret => ⌜vret = Vundef↑⌝ ** OwnM Run))).
 
   Definition loop_spec: fspec :=
